commit

Src/Prover/Main.lean
@@ -12,13 +12,13 @@ theorem not_mem_of_empty {a b} (h : empty a) : b ∉ a :=
 theorem empty_iff {a} : empty a ↔ ∀ b, b ∉ a :=
 iff_intro (λ h _ => not_mem_of_empty h) (λ h h₁ => exi_elim h₁ h)
 
-theorem nempty_intro {a} b (h : b ∈ a) : nempty a :=
+theorem nonempty_intro {a} b (h : b ∈ a) : nonempty a :=
 not_not_intro # exi_intro b h
 
-theorem nempty_elim {P : Prop} {a} (h₁ : nempty a) (h₂ : ∀ b, b ∈ a → P) : P :=
+theorem nonempty_elim {P : Prop} {a} (h₁ : nonempty a) (h₂ : ∀ b, b ∈ a → P) : P :=
 exi_elim (not_not_elim h₁) h₂
 
-theorem nempty_iff {a} : nempty a ↔ ∃ b, b ∈ a :=
+theorem nonempty_iff {a} : nonempty a ↔ ∃ b, b ∈ a :=
 iff_intro not_not_elim not_not_intro
 
 theorem exi_empty : ∃ a, empty a :=
@@ -32,9 +32,9 @@ notation (priority := high) "∅" => emp
 theorem empty_emp : empty ∅ :=
 some_spec exi_empty
 
-theorem exi_nempty : ∃ a, nempty a :=
+theorem exi_nonempty : ∃ a, nonempty a :=
 exi_elim ax_inf # λ a h₁ => exi_elim h₁ # λ b h₂ => exi_intro a #
-nempty_intro b # and_left # and_right h₂
+nonempty_intro b # and_left # and_right h₂
 
 def filter (a : Set) (P : Set → Prop) : Set :=
 some # ax_spec a P
@@ -73,30 +73,30 @@ iff_intro
 (λ h => mpr mem_filter # and_intro (mem_image_aux_of h) h)
 
 def singleton (a : Set) : Set :=
-image (some exi_nempty) # λ b => a
+image (some exi_nonempty) # λ b => a
 
 theorem mem_singleton {a b} : b ∈ singleton a ↔ b = a :=
 iff_intro
 (λ h => exi_elim (mp mem_image h) # λ c h₁ => eq_symm # and_right h₁)
-(λ h => mpr mem_image # exi_elim (mp nempty_iff # some_spec exi_nempty) #
+(λ h => mpr mem_image # exi_elim (mp nonempty_iff # some_spec exi_nonempty) #
   λ c h₁ => exi_intro c # and_intro h₁ # eq_symm h)
 
 theorem mem_singleton_self {a} : a ∈ singleton a :=
 mpr mem_singleton rfl
 
-theorem nempty_singleton {a} : nempty (singleton a) :=
-nempty_intro a mem_singleton_self
+theorem nonempty_singleton {a} : nonempty (singleton a) :=
+nonempty_intro a mem_singleton_self
 
 theorem mem_irrefl {a} : a ∉ a :=
-exi_elim (ax_reg nempty_singleton) # λ b h => and_elim h # λ h₁ h₂ h₃ => h₂ #
+exi_elim (ax_reg nonempty_singleton) # λ b h => and_elim h # λ h₁ h₂ h₃ => h₂ #
 exi_intro a # and_intro (eq_rec' (λ x => a ∈ x) (mp mem_singleton h₁) h₃)
 mem_singleton_self
 
-theorem nempty_image {a} {f : Set → Set} : nempty (image a f) ↔ nempty a :=
+theorem nonempty_image {a} {f : Set → Set} : nonempty (image a f) ↔ nonempty a :=
 iff_intro
-(λ h => nempty_elim h # λ b h₁ => exi_elim (mp mem_image h₁) #
-  λ c h₂ => nempty_intro c # and_left h₂)
-(λ h => nempty_elim h # λ b h₁ => nempty_intro (f b) # mpr mem_image #
+(λ h => nonempty_elim h # λ b h₁ => exi_elim (mp mem_image h₁) #
+  λ c h₂ => nonempty_intro c # and_left h₂)
+(λ h => nonempty_elim h # λ b h₁ => nonempty_intro (f b) # mpr mem_image #
   exi_intro b # and_intro h₁ rfl)
 
 theorem not_mem_emp {a} : a ∉ ∅ :=
@@ -105,7 +105,7 @@ not_mem_of_empty empty_emp
 theorem empty_iff_eq_emp {a} : empty a ↔ a = ∅ :=
 iff_intro
 (λ h => ax_ext # λ b => iff_intro
-  (λ h₁ => false_elim # not_mem_of_empty h h₁) (λ h₁ => false_elim # not_mem_emp h₁))
+  (λ h₁ => exfalso # not_mem_of_empty h h₁) (λ h₁ => exfalso # not_mem_emp h₁))
 (λ h => eq_rec' empty h empty_emp)
 
 def some_inf : Set :=
@@ -116,30 +116,38 @@ exi_elim (some_spec ax_inf) # λ d h =>
 eq_rec (λ x => x ∈ some_inf) (mp empty_iff_eq_emp # and_left h) #
 and_left # and_right h
 
-theorem nempty_some_inf : nempty some_inf :=
-nempty_intro ∅ emp_mem_some_inf
+theorem nonempty_some_inf : nonempty some_inf :=
+nonempty_intro ∅ emp_mem_some_inf
 
 theorem ne_singleton_self {a} : a ≠ singleton a :=
 λ h => mem_irrefl # eq_symm h (λ x => a ∈ x) mem_singleton_self
 
-def pwset (a : Set) : Set :=
+def powerset (a : Set) : Set :=
 filter (some # ax_pow a) # λ b => b ⊆ a
 
-theorem mem_pwset {a b} : b ∈ pwset a ↔ b ⊆ a :=
+theorem mem_powerset {a b} : b ∈ powerset a ↔ b ⊆ a :=
 iff_intro
 (λ h => and_right (mp (@mem_filter (λ x => x ⊆ a) _ _) h))
 (λ h => mpr mem_filter # and_intro (some_spec (ax_pow a) b h) h)
 
-theorem mem_pwset_self {a} : a ∈ pwset a :=
-mpr mem_pwset subset_refl
+theorem mem_powerset_self {a} : a ∈ powerset a :=
+mpr mem_powerset subset_refl
+
+theorem eq_iff_mem {a b} : a = b ↔ ∀ c, c ∈ a ↔ c ∈ b :=
+iff_intro
+(λ h c => mp eq_iff h (λ x => c ∈ x))
+(λ h => ax_ext h)
+
+theorem ne_powerset_self {a} : a ≠ powerset a :=
+λ h => @mem_irrefl a # mpr (mp eq_iff_mem h a) mem_powerset_self
 
 section Conditional
 
 theorem exi_ite_val {α : Type} (P : Prop) (x y : α) :
   ∃ (z : α), (P → z = x) ∧ (¬P → z = y) :=
 prop_rec (λ m => ∃ (z : α), (m → z = x) ∧ (¬m → z = y))
-(exi_intro x # and_intro (λ _ => rfl) (λ h => false_elim # h trivial))
-(exi_intro y # and_intro false_elim (λ _ => rfl))
+(exi_intro x # and_intro (λ _ => rfl) (λ h => exfalso # h trivial))
+(exi_intro y # and_intro exfalso (λ _ => rfl))
 
 def ite {α : Type} (P : Prop) (x y : α) : α :=
 some # exi_ite_val P x y
@@ -171,43 +179,43 @@ theorem not_mem_zero {a} : a ∉ 0 :=
 not_mem_emp
 
 def one : Set :=
-pwset 0
+powerset 0
 
 instance : OfNat Set (nat_lit 1) := ⟨one⟩
 
 theorem zero_mem_one : 0 ∈ 1 :=
-mem_pwset_self
+mem_powerset_self
 
-theorem nempty_one : nempty 1 :=
-nempty_intro 0 zero_mem_one
+theorem nonempty_one : nonempty 1 :=
+nonempty_intro 0 zero_mem_one
 
 theorem subset_emp {a} : a ⊆ ∅ ↔ a = ∅ :=
 iff_intro
-(λ h => mp empty_iff_eq_emp # contra # λ h₁ => nempty_elim (mp not_empty h₁) #
+(λ h => mp empty_iff_eq_emp # contra # λ h₁ => nonempty_elim (mp not_empty h₁) #
   λ b h₂ => not_mem_emp # h b h₂)
 (λ h => eq_rec' (λ x => x ⊆ ∅) h subset_refl)
 
 theorem mem_one {a} : a ∈ 1 ↔ a = 0 :=
 iff_intro
-(λ h => mp subset_emp # mp mem_pwset h)
+(λ h => mp subset_emp # mp mem_powerset h)
 (λ h => eq_rec' (λ x => x ∈ 1) h zero_mem_one)
 
 def two : Set :=
-pwset 1
+powerset 1
 
 instance : OfNat Set (nat_lit 2) := ⟨two⟩
 
 theorem emp_subset {a} : ∅ ⊆ a :=
-λ b h => false_elim # not_mem_emp h
+λ b h => exfalso # not_mem_emp h
 
-theorem emp_mem_pwset {a} : emp ∈ pwset a :=
-mpr mem_pwset emp_subset
+theorem emp_mem_powerset {a} : emp ∈ powerset a :=
+mpr mem_powerset emp_subset
 
 theorem zero_mem_two : 0 ∈ 2 :=
-emp_mem_pwset
+emp_mem_powerset
 
 theorem one_mem_two : 1 ∈ 2 :=
-mpr mem_pwset subset_refl
+mpr mem_powerset subset_refl
 
 theorem zero_ne_one : (0 : Set) ≠ 1 :=
 λ h => mem_irrefl # mpr (mp eq_iff h (λ x => 0 ∈ x)) zero_mem_one
@@ -218,11 +226,6 @@ theorem zero_ne_two : (0 : Set) ≠ 2 :=
 theorem one_ne_two : (1 : Set) ≠ 2 :=
 λ h => mem_irrefl # mpr (mp eq_iff h (λ x => 1 ∈ x)) one_mem_two
 
-theorem eq_iff_mem {a b} : a = b ↔ ∀ c, c ∈ a ↔ c ∈ b :=
-iff_intro
-(λ h c => mp eq_iff h (λ x => c ∈ x))
-(λ h => ax_ext h)
-
 theorem one_eq_singleton_zero : 1 = singleton 0 :=
 mpr eq_iff_mem # λ a => iff_rec' (λ x => x ↔ a ∈ singleton 0) mem_one #
 iff_rec' (λ x => a = 0 ↔ x) mem_singleton iff_refl
@@ -231,7 +234,7 @@ def subsingleton (a : Set) : Prop :=
 ∀ (b c : Set), b ∈ a → c ∈ a → b = c
 
 theorem subsingleton_emp : subsingleton ∅ :=
-λ b c h => false_elim # not_mem_emp h
+λ b c h => exfalso # not_mem_emp h
 
 theorem subsingleton_singleton {a} : subsingleton (singleton a) :=
 λ b c h₁ h₂ => eq_trans (mp mem_singleton h₁) (eq_symm # mp mem_singleton h₂)
@@ -246,7 +249,7 @@ theorem subsingleton_iff {a} : subsingleton a ↔ a = ∅ ∨ ∃ b, a = singlet
 iff_intro
 (λ h => by_cases (empty a)
   (λ h₁ => or_inl # mp empty_iff_eq_emp h₁)
-  (λ h₁ => or_inr # nempty_elim (mp not_empty h₁) # λ b h₂ => exi_intro b #
+  (λ h₁ => or_inr # nonempty_elim (mp not_empty h₁) # λ b h₂ => exi_intro b #
     mpr eq_iff_mem # λ c => iff_rec' (λ x => c ∈ a ↔ x) mem_singleton # iff_intro
       (λ h₃ => h c b h₃ h₂) (λ h₃ => eq_rec' (λ x => x ∈ a) h₃ h₂)))
 (λ h => or_elim h
@@ -263,9 +266,9 @@ theorem subset_singleton {a b} : b ⊆ singleton a ↔ b = ∅ ∨ b = singleton
 iff_intro
 (λ h => by_cases (empty b)
   (λ h₂ => or_inl # mp empty_iff_eq_emp h₂)
-  (λ h₂ => or_inr # nempty_elim (mp not_empty h₂) # λ c h₃ => mpr eq_iff_mem # λ d =>
-    iff_intro (h d) # λ h₄ => eq_rec' (λ x => x ∈ b) (mp mem_singleton h₄) #
-      eq_rec' (λ x => x ∈ b) (eq_symm # mp mem_singleton # h c h₃) h₃))
+  (λ h₂ => or_inr # nonempty_elim (mp not_empty h₂) # λ c h₃ => mpr eq_iff_mem # λ d =>
+    iff_intro (h d) # λ h₄ => eq_rec' (λ x => x ∈ b)
+      (eq_trans (mp mem_singleton h₄) (eq_symm # mp mem_singleton # h c h₃)) h₃))
 (λ h => or_elim h
   (λ h₁ => eq_rec' (λ x => x ⊆ singleton a) h₁ emp_subset)
   (λ h₁ => eq_rec' (λ x => x ⊆ singleton a) h₁ subset_refl))
@@ -278,12 +281,12 @@ iff_intro
   (λ h₂ => eq_rec' (λ x => x ⊆ a) h₂ emp_subset)
   (λ h₂ => eq_rec' (λ x => x ⊆ a) h₂ subset_refl))
 
-theorem mem_pwset_of_subsingleton {a b} (h : subsingleton a) :
-  b ∈ pwset a ↔ b = ∅ ∨ b = a :=
-iff_rec' (λ x => x ↔ b = ∅ ∨ b = a) mem_pwset # subset_of_subsingleton h
+theorem mem_powerset_of_subsingleton {a b} (h : subsingleton a) :
+  b ∈ powerset a ↔ b = ∅ ∨ b = a :=
+iff_rec' (λ x => x ↔ b = ∅ ∨ b = a) mem_powerset # subset_of_subsingleton h
 
 theorem mem_two {a} : a ∈ 2 ↔ a = 0 ∨ a = 1 :=
-mem_pwset_of_subsingleton subsingleton_one
+mem_powerset_of_subsingleton subsingleton_one
 
 end Natural_numbers
 
@@ -295,15 +298,15 @@ image some_inf # λ c => ite (empty c) a b
 theorem empty_elim (P : Set → Prop) {a} (h₁ : empty a) (h₂ : P ∅) : P a :=
 eq_rec' P (mp empty_iff_eq_emp h₁) h₂
 
-theorem nempty_upair {a b : Set} : nempty (upair a b) :=
-mpr nempty_image # nempty_some_inf
+theorem nonempty_upair {a b : Set} : nonempty (upair a b) :=
+mpr nonempty_image # nonempty_some_inf
 
 theorem zero_mem_some_inf : 0 ∈ some_inf :=
 emp_mem_some_inf
 
 theorem is_succ_one_zero : is_succ 1 0 :=
 λ a => iff_intro (λ h => or_inr # mp mem_one h)
-(λ h => or_elim h (λ h₁ => false_elim # not_mem_zero h₁) (mpr mem_one))
+(λ h => or_elim h (λ h₁ => exfalso # not_mem_zero h₁) (mpr mem_one))
 
 theorem one_mem_some_inf : 1 ∈ some_inf :=
 exi_elim (some_spec ax_inf) # λ a h => and_right (and_right h) 0
@@ -317,9 +320,46 @@ iff_intro
   (λ h₁ => exi_intro ∅ # and_intro emp_mem_some_inf #
     eq_trans (if_pos empty_emp) (eq_symm h₁))
   (λ h₁ => exi_intro 1 # and_intro one_mem_some_inf #
-    eq_rec' (λ x => ite (empty 1) a b = x) h₁ # if_neg # mpr not_empty nempty_one))
+    eq_rec' (λ x => ite (empty 1) a b = x) h₁ # if_neg # mpr not_empty nonempty_one))
+
+theorem upair_comm {a b} : upair a b = upair b a :=
+mpr eq_iff_mem # λ c => iff_rec' (λ x => x ↔ _) mem_upair #
+iff_rec' (λ x => _ ↔ x) mem_upair or_symm'
+
+theorem upair_self_eq {a} : upair a a = singleton a :=
+mpr eq_iff_mem # λ b => iff_rec' (λ x => x ↔ _) (iff_trans mem_upair or_self) #
+iff_rec' (λ x => _ ↔ x) mem_singleton iff_refl
+
+theorem subsingleton_upair_iff {a b} : subsingleton (upair a b) ↔ a = b :=
+iff_intro
+(λ h => or_elim (mp subsingleton_iff h)
+  (λ h₁ => exfalso # mpr not_nonempty (mpr empty_iff_eq_emp h₁) nonempty_upair)
+  (λ h₁ => exi_elim h₁ # λ c h₂ => eq_trans' c
+    (mp mem_singleton # mp (mp eq_iff_mem h₂ a) # mpr mem_upair # or_inl rfl)
+    (eq_symm # mp mem_singleton # mp (mp eq_iff_mem h₂ b) #
+       mpr mem_upair # or_inr rfl)))
+(λ h => eq_rec' (λ x => subsingleton (upair x b)) h #
+  eq_rec' subsingleton upair_self_eq subsingleton_singleton)
 
 end Unordered_pair
 
-theorem ne_pwset_self {a} : a ≠ pwset a :=
-λ h => @mem_irrefl a # mpr (mp eq_iff_mem h a) mem_pwset_self
+section Ordered_pair
+
+def pair (a b : Set) : Set :=
+upair a (upair a b)
+
+theorem eq_left_of_pair_eq_pair {a b c d} (h : pair a b = pair c d) : a = c :=
+sorry
+
+theorem eq_right_of_pair_eq_pair {a b c d} (h : pair a b = pair c d) : b = d :=
+sorry
+
+theorem eq_and_eq_of_pair_eq_pair {a b c d} (h : pair a b = pair c d) : a = c ∧ b = d :=
+and_intro (eq_left_of_pair_eq_pair h) (eq_right_of_pair_eq_pair h)
+
+theorem pair_ext {a b c d} : pair a b = pair c d ↔ a = c ∧ b = d :=
+iff_intro eq_and_eq_of_pair_eq_pair #
+λ h₁ => eq_rec' (λ x => pair x b = pair c d) (and_left h₁) #
+eq_rec' (λ x => pair c x = pair c d) (and_right h₁) rfl
+
+end Ordered_pair
